formal/pickles/Pickles.lean
@@ -7,6 +7,7 @@ import Pickles.OptSponge
 import Pickles.FrSponge
 import Pickles.Pseudo
 import Pickles.Domain
+import Pickles.Statement
 import Pickles.FinalizeOtherProof
 import Pickles.FqSpongeTranscript
 import Pickles.CheckBulletproof
